theory.lean
@@ -3,6 +3,20 @@
 inference and synthesis for unityped languages
 -/
 
+-- problem 
+/-
+- synthesize terms from context with missing type annotations in a dynamic language
+  - infer actual types from terms  
+    - inference for all term cases
+    - solve typing constraints locally
+      - accept all constraints where expected type is unbounded (top) 
+      - maintain leniency of expected type while 
+        - recording previously seen types (ty | ?)
+        - bounding actual types (ty | ?)
+      - reject constraints with contradictions without  
+
+  - synthesize terms from local types 
+-/
 
 -- background
 /-
@@ -68,6 +82,15 @@ inference and synthesis for unityped languages
 - [x] learn PHOAS for pattern matching
 - [x] learn macros in Lean 
 - [_] learn termination for PHOAS in Lean 
+  - difficulty due to mutual inductive defs and Sigma
+- [_] determine how to represent bound variables 
+  - locally nameless de bruijn
+- [_] determine how to represent free variables
+  - free var natural number
+    - natural number = 1 + max(prev natural numbers)
+    - assoc list of (free var, type) independent of term
+  - dependent phoas / de bruijn: all variables are free with a local context
+
 - consider adding relative complement type 
   - i.e. binary negation type operator
   - i.e. (τ₁ \ τ₂) ≤ (τ₁ & ¬ τ₂), where ⊤ / τ₂ = ¬ τ₂)
@@ -79,6 +102,1229 @@ inference and synthesis for unityped languages
   - refinement types vs unityped subtyping
   - solution
   - evidence
+-/
+
+-- syntax 
+/-
+α ∈ terminal                      type variable
+l ∈ terminal                      label
+
+Δ ::=                             subtyping environment 
+  ⬝                                empty
+  Δ ; α ≤ τ                       extension
+
+τ ::=                             type
+  ?                               unknown
+  α                               variable
+  []                              unit
+  #l τ                            variant
+  .l τ                            field
+  τ | τ                           union
+  τ & τ                           intersection
+  τ -> τ                          func 
+  ∀ Δ C τ                         universal schema 
+  μ α . τ                         induction
+  [τ]                             group
+
+C ::=                             constraint
+  .                               true
+  ⟨C⟩                             grouped constraint 
+  τ ≤ τ                           subtyping 
+  C ∨ C                           disjunction
+  C ∧ C                           conjunction
+
+-/
+
+mutual 
+  inductive Ty : Type
+    | unknown : Ty
+    | bvar : Nat -> Ty  
+    | fvar : Nat -> Ty
+    | unit : Ty
+    | variant : String -> Ty -> Ty
+    | field : String -> Ty -> Ty
+    | union : Ty -> Ty -> Ty
+    | inter : Ty -> Ty -> Ty
+    | func : Ty -> Ty -> Ty
+    | univ : List Ty -> Constr -> Ty -> Ty
+    | induct : Ty -> Ty
+
+  inductive Constr : Type
+    | tru : Constr
+    | subtype : Ty -> Ty -> Constr
+    | disj : Constr -> Constr -> Constr
+    | conj : Constr -> Constr -> Constr
+end
+
+
+declare_syntax_cat slm
+syntax num : slm 
+syntax ident : slm
+syntax "[" slm,+ "]" : slm 
+syntax "£"slm:90 : slm
+syntax "@"slm:90 : slm
+syntax "#"slm:90 slm : slm
+syntax "."slm:90 slm : slm
+syntax "(_)" : slm
+syntax "(-)" : slm
+syntax "(=)" : slm
+syntax "?" : slm
+syntax:50 slm:50 "->" slm:51 : slm
+syntax:60 slm:60 "|" slm:61 : slm
+syntax:70 slm:70 "&" slm:71 : slm
+syntax "∀" slm slm "." slm : slm 
+syntax "∀" slm "." slm : slm 
+syntax "μ 0 ." slm : slm 
+
+syntax:30 slm:30 "∨" slm:31 : slm
+syntax:40 slm:40 "∧" slm:41 : slm
+syntax:50 slm:50 "≤" slm:51 : slm
+
+syntax "(" slm ")" : slm
+
+syntax "⟨" term "⟩" : slm 
+
+syntax "[: " slm ":]" : term
+
+macro_rules
+
+-- terminals
+  | `([: $n:num :]) => `($n)
+  | `([: $a:ident:]) => `($(Lean.quote (toString a.getId)))
+-- context 
+  | `([: [$x:slm] :]) => `([ [: $x :] ])
+  | `([: [$x,$xs:slm,*] :]) => `([: $x :] :: [: [$xs,*] :])
+-- Ty 
+  | `([: £$n :]) => `(Ty.bvar [: $n :])
+  | `([: @$n:slm :]) => `(Ty.fvar [: $n :])
+  | `([: #$a $b:slm :]) => `(Ty.variant [: $a :] [: $b :])
+  | `([: .$a $b:slm :]) => `(Ty.field [: $a :] [: $b :])
+  | `([: ? :]) => `(Ty.unknown)
+  | `([: $a -> $b :]) => `(Ty.func [: $a :] [: $b :])
+  | `([: $a | $b :]) => `(Ty.union [: $a :] [: $b :])
+  | `([: $a & $b :]) => `(Ty.inter [: $a :] [: $b :])
+  | `([: ∀ $a:slm $b:slm . $c:slm :]) => `(Ty.univ [: $a :] [: $b :] [: $c :])
+  | `([: ∀ $a:slm . $b:slm :]) => `(Ty.univ [: $a :] [: (=) :] [: $b :] )
+  | `([: μ 0 . $a :]) => `(Ty.induct [: $a :])
+  | `([: (-) :]) => `(Ty.unit)
+-- Constr
+  | `([: (=) :]) => `(Constr.tru)
+  | `([: $a:slm ≤ $b:slm :]) => `(Constr.subtype [: $a :] [: $b :])
+  | `([: $a ∨ $b :]) => `(Constr.disj [: $a :] [: $b :])
+  | `([: $a ∧ $b :]) => `(Constr.conj [: $a :] [: $b :])
+
+-- generic
+  | `([: ($a) :]) => `([: $a :])
+
+--escape 
+  | `([: ⟨ $e ⟩ :]) => pure e
+
+
+-- #check [: @⟨1⟩ :]
+
+
+def z := 1
+#check [: @⟨z⟩ :]
+def x := Ty.bvar 1
+
+
+#check [: £0 & ? :]
+#check [: ∀ [?] (=) . ⟨x⟩ :]
+#check [: ∀ [?] (=) . £0 :]
+#check [: ∀ [?, ?] (=) . £0 :]
+#check [: ∀ [?, ?] . £0 :]
+#check [: (-) :]
+#check [: @24 :]
+#check [: #foo ? | #boo ? :]
+#check [: μ 0 . #foo £0 :]
+#check [: μ 0 . #foo £0  & ? | @2 & ?:]
+#check [: £3 & ? -> @1 | @2 :]
+#check [: μ 0 . #foo £0  & ? | @2 & ? -> @1 | @2 :]
+#check [: μ 0 . #foo £0  & ? | @2 & ? :]
+#check [: ? :]
+#check [: (=) ∧ (=) :]
+#check [: ? ≤ ? & £0 ∧ (=) :]
+
+mutual 
+  inductive Ty.has_size : Ty -> Nat -> Type
+    | unknown : Ty.has_size Ty.unknown 0 
+    | bvar : Ty.has_size (Ty.bvar _) 0 
+    | fvar : Ty.has_size (Ty.fvar _) 0 
+    | unit : Ty.has_size (Ty.unit) 0 
+    | variant : Ty.has_size ty n -> Ty.has_size (Ty.variant _ ty) (n + 1) 
+    | field : Ty.has_size ty n -> Ty.has_size (Ty.field _ ty) (n + 1) 
+    | union : Ty.has_size ty₁ n₁ -> Ty.has_size ty₂ n₂ -> Ty.has_size (.union ty₁ ty₂) (n₁ + n₂ + 1)
+    | inter : Ty.has_size ty₁ n₁ -> Ty.has_size ty₂ n₂ -> Ty.has_size (.inter ty₁ ty₂) (n₁ + n₂ + 1)
+    | func : Ty.has_size ty₁ n₁ -> Ty.has_size ty₂ n₂ -> Ty.has_size (.func ty₁ ty₂) (n₁ + n₂ + 1)
+    | univ : ListTy.has_size ctx ns -> Constr.has_size c n_ty -> Ty.has_size ty n_ty -> 
+        Ty.has_size (Ty.univ ctx c ty) (ns + n_c + n_ty + 1)
+    | induct : Ty.has_size ty n -> Ty.has_size (Ty.induct ty) (n + 1) 
+
+  inductive ListTy.has_size : (List Ty) -> Nat -> Type
+    | nil : 
+        ListTy.has_size [] 0
+    | cons : 
+        Ty.has_size ty n_ty -> 
+        ListTy.has_size tys n_tys -> 
+        ListTy.has_size (ty::tys) (n_tys + n_ty)
+
+  inductive Constr.has_size : Constr -> Nat -> Type
+    | tru : 
+        Constr.has_size Constr.tru 0  
+    | subtype : 
+        Ty.has_size ty₁ n₁ -> Ty.has_size ty₂ n₂ -> 
+        Constr.has_size (Constr.subtype ty₁ ty₂) (n₁ + n₂ + 1) 
+    | disj :
+        Constr.has_size c₁ n₁ -> Constr.has_size c₂ n₂ -> 
+        Constr.has_size (Constr.disj ty₁ ty₂) (n₁ + n₂ + 1) 
+    | conj :
+        Constr.has_size c₁ n₁ -> Constr.has_size c₂ n₂ -> 
+        Constr.has_size (Constr.disj ty₁ ty₂) (n₁ + n₂ + 1) 
+end
+
+
+#check Nat.lt
+
+@[reducible] def Ty.lt (ty₁ : Ty) (ty₂ : Ty) : Prop := 
+  ∀ n₁ n₂ , Ty.has_size ty₁ n₁ -> Ty.has_size ty₂ n₂ -> n₁ < n₂
+
+example : ¬ Ty.lt Ty.unknown Ty.unknown := 
+  ((fun h =>
+    let f := h 0 0 
+    let w := f Ty.has_size.unknown Ty.has_size.unknown
+    let z := Nat.ne_of_lt w
+    absurd rfl z
+  ))
+
+example : ¬ Ty.lt Ty.unknown Ty.unknown := by
+  unfold Ty.lt
+  intro h 
+  generalize (h 0 0) = f 
+  generalize (f Ty.has_size.unknown Ty.has_size.unknown) = w 
+  generalize Nat.ne_of_lt w = z
+  apply absurd (rfl) z 
+
+-- def Ty.acc : (a : Ty) -> Acc lt a
+
+-- theorem Ty.wf : WellFounded Ty.lt := 
+--   (WellFounded.intro (fun 
+--     | Ty.unknwon => Acc.intro 
+--   ))
+
+
+
+def Constr.lt (c₁ : Constr) (c₂ : Constr) : Prop := 
+  ∀ n₁ n₂ , Constr.has_size c₁ n₁ -> Constr.has_size c₂ n₂ -> n₁ < n₂
+
+#check Sum
+#check ((Sum.inl 1)) 
+
+def TyConstr.lt (p₁ : (Sum Ty Constr)) (p₂ : Sum Ty Constr) : Prop :=
+  match (p₁, p₂) with
+    | (Sum.inl ty₁, Sum.inl ty₂) =>  Ty.lt ty₁ ty₂
+    | (.inl ty₁, .inr c₂)  =>
+        ∀ n₁ n₂ , Ty.has_size ty₁ n₁ -> Constr.has_size c₂ n₂ -> n₁ < n₂
+    | (.inr c₁, .inl ty₂) =>
+        ∀ n₁ n₂ , Constr.has_size c₁ n₁ -> Ty.has_size ty₂ n₂ -> n₁ < n₂
+    | (.inr c₁, .inr c₂) => Constr.lt c₁ c₂ 
+
+
+-- instance : WellFoundedRelation (Sum Ty Constr) where
+--   rel := TyConstr.lt 
+--   wf :=  
+
+
+/-
+x ∈ terminal                      term variable
+
+p ::=                             term
+  _                               hole
+  x                               variable
+  ()                              unit
+  #l p                            variant
+  ps                              record
+
+ps ::=                            fields 
+  .l p                            field singleton 
+  ps .l p                         fields extended 
+-/
+
+
+mutual
+  inductive Pat : (T : Type) -> Nat -> Type where
+    | hole : Pat T 0 
+    | bvar : T -> Ty -> Pat T 1
+    | unit : Pat T 0 
+    | variant : String -> Pat T 0 
+    | record {n : Nat} : PatRec T n -> Pat T n 
+
+  inductive PatRec : (T : Type) -> Nat -> Type where
+    | single {n : Nat} : String -> Pat T n -> PatRec T n 
+    | exten {n₁ n₂ : Nat} : String -> Pat T n₁ -> PatRec T n₂-> PatRec T (n₁ + n₂)
+end
+
+/-
+t ::=                             term
+  _                               hole 
+  x                               variable
+  ()                              unit
+  #l t                            variant
+  fs                              record
+  cs                              function
+  t.l                             projection
+  t t                             application
+  let x : τ = t in t              binding
+  fix t                           recursion
+
+cs ::=                            cases
+  for p => t                      singleton 
+  cs for p => t                   extension 
+
+fs ::=                            fields 
+  .l t                            singleton 
+  fs .l t                         extension
+-/
+
+mutual
+  inductive Tm (T : Type): Type
+    | hole : Tm T 
+    | bvar : T -> Tm T 
+    | fvar : Nat -> Tm T 
+    | unit : Tm T
+    | variant : String -> Tm T -> Tm T
+    | record : List (String × Tm T) -> Tm T
+    | func : List (Σ n, Case T n) -> Tm T
+    | proj : Tm T -> String -> Tm T
+    | app : Tm T -> Tm T -> Tm T
+    | letb : Tm T -> Ty -> (T -> Tm T) -> Tm T
+    | fix : Tm T -> Tm T
+
+  inductive Case (T : Type) : Nat -> Type
+    | mk {n : Nat} : Pat T n -> Tm T -> Case T n
+
+end
+
+
+/-
+
+m ::=                             substitution map
+  ⬝                                empty
+  α / τ :: m                      extension
+
+Γ ::=                             typing environment 
+  ⬝                                empty
+  x : τ :: Γ                      extension
+
+-/
+
+
+
+
+-- dynamic semantics 
+/-
+-/
+
+-- dynamic implementation 
+/-
+beyond scope
+-/
+
+-- dynamic semantics/implementation theorems
+/-
+beyond scope
+-/
+
+-- static semantics 
+/-
+
+consistent constraint subtyping   
+`Δ ⊢ C`
+```
+Δ ⊢ .
+
+  Δ ⊢ C 
+---
+Δ ⊢ ⟨C⟩ 
+
+  Δ ⊢ C₁ 
+  Δ ⊢ C₂
+---
+Δ ⊢ C₁ ∧ C₂ 
+
+  Δ ⊢ C₁ 
+---
+Δ ⊢ C₁ ∨ C₂ 
+
+  Δ ⊢ C₂
+---
+Δ ⊢ C₁ ∨ C₂ 
+
+Δ ⊢ τ ≤ τ
+
+Δ ⊢ τ ≤ ? 
+
+Δ ⊢ ? ≤ τ 
+
+  Γ ⊢ τ' ≤ τₘ
+  Γ ⊢ τₘ ≤ τ
+  τₘ ≠ ?
+---
+Δ ⊢ τ' ≤ τ  
+
+
+  {α ≤ τ} ⊆ Δ
+---
+Δ ⊢ α ≤ τ  
+
+
+  Δ₀, Δ' ⊢ C' ∧ τ' ≤ τ
+---
+Δ₀ ⊢ (∀ Δ' C' τ') ≤ τ
+
+
+  Δ₀, Δ ⊢ C ∧ τ' ≤ τ
+---
+Δ₀ ⊢ τ' ≤ (∀ Δ C τ)
+
+
+Δ₀ ⊢ (μ α . τ) ≤ unroll (μ α . τ)
+
+
+Δ₀ ⊢ unroll (μ α . τ) ≤ (μ α . τ)
+
+
+  Δ ⊢ τ₁' ≤ τ₁ 
+  Δ ⊢ τ₂' ≤ τ₂ 
+---
+Δ ⊢ τ₁ -> τ₂' ≤ τ₁' -> τ₂
+
+
+  Δ ⊢ τ' ≤ τ
+---
+Δ ⊢ .l τ' ≤ .l τ  
+
+
+  Δ ⊢ τ' ≤ τ  
+---
+Δ ⊢ #l τ' ≤ #l τ
+
+
+Δ ⊢ τ' ≤ (τ' | τ)  
+
+Δ ⊢ τ' ≤ (τ | τ')  
+
+
+  Δ ⊢ τ₁ ≤ τ   
+  Δ ⊢ τ₂ ≤ τ  
+---
+Δ ⊢ (τ₁ | τ₂) ≤ τ 
+
+
+Δ ⊢ (τ & τ') ≤ τ
+
+Δ ⊢ (τ' & τ) ≤ τ  
+
+
+  Δ ⊢ τ' ≤ τ₁  
+  Δ ⊢ τ' ≤ τ₂  
+---
+Δ ⊢ τ' ≤ τ₁ & τ₂  
+```
+
+constraint typing  
+`Γ Δ C ⊢ t : τ`
+```
+TODO: fill in constraint typing rules
+```
+
+-/
+
+-- static implementation 
+/-
+
+
+`merge Δ Δ = Δ`
+```
+merge op Δ₁ Δ₂ =
+  fmap Δ₁ (α ≤ τ₁ =>
+  fmap Δ₂ (β ≤ τ₂ =>
+    {α ≤ τ₁ op (Δ₂ α), β ≤ (Δ₁ β) op τ₂}
+  ))
+```
+
+`merge o[Δ] o[Δ] = o[Δ]`
+```
+merge _ none none = none 
+merge _ none o = o 
+merge _ o none = o 
+merge op (some Δ₁) (some Δ₂) = some (merge op Δ₁ Δ₂)
+```
+-/
+
+
+def lookup (key : Nat) : List (Nat × T) -> Option T
+  | (k,v) :: bs => if key = k then some v else lookup key bs 
+  | [] => none
+
+
+#check List.bind
+partial def merge (op : T -> T -> T) (df : T) (Δ₁ : List (Nat × T))  (Δ₂ : List (Nat × T)) : List (Nat × T) :=
+  List.bind Δ₁ (fun (key₁, v₁) =>
+  List.bind Δ₂ (fun (key₂, v₂) =>
+    let uno := match lookup key₁ Δ₂ with
+      | Option.some v₂ => [(key₁, op v₁ v₂)]
+      | Option.none => [(key₁, op v₁ df)] 
+
+    let dos := match lookup key₂ Δ₁ with
+      | Option.some _ => [] 
+      | Option.none => [(key₂, op v₂ df)]
+    uno ++ dos
+  ))
+
+
+/-
+
+
+`linearize_record τ = o[fs]`
+```
+linearize_record .l₁ τ₁ & .l₂ τ₂ =
+  some (.l₁ τ₁ & .l₂ τ₂)
+linearize_record .l τ₁ & τ₂ =
+  some .l τ₁ & (linearize_record τ₂)
+linearize_record τ₁ & .l τ₂ =
+  some .l τ₂ & (linearize_record τ₁)
+linearize_record τ₁ & τ₂ =
+  none
+```
+
+`make_record_constraint Δ ⊢ τ * τ ≤ τ = o[C]`
+```
+make_record_constraint Δ ⊢ τ₀ * .l τ₁ & τ₂ ≤ μ α . τ =
+  let β₁ = fresh in
+  let C₁ = τ₁ ≤ ∀ {β₁ ≤ ?} ⟨(τ₀ & .l β₁ & τ₂) ≤ unroll (μ α . τ)⟩ . β₁ in
+  C₁ ∧ make_record_constraint (Δ ⊢ τ₀ & .l τ₁ * τ₂ ≤ μ α . τ)
+
+make_record_constraint Δ ⊢ τ₀ * .l τ₁ ≤ μ α . τ =
+  let β₁ = fresh in
+  let C₁ = τ₁ ≤ ∀ {β₁ ≤ ?} ⟨(τ₀ & .l β₁) ≤ unroll (μ α . τ)⟩ . β₁ in
+  C₁
+
+make_record_constraint _ ⊢ _ * _ ≤ _ = none
+```
+
+`match o o = b`
+```
+match (some x₁) (some ×₂) = 
+  x₁ = x₂
+match none _ = false
+match _ none = false
+```
+
+`cases_normal τ τ = b`
+```
+cases_normal (#l₁ τ₁) (#l₂ τ₂) = true
+cases_normal τ₁ τ₂ = 
+  fmap (keys τ₁) (ks₁ =>
+  fmap (keys τ₂) (ks₂ =>
+    some (ks₁ = ks₂)
+  )) = Some true
+  (keys τ₁) = (keys τ₂) 
+```
+
+
+`decreasing τ τ = b`
+```
+decreasing (#l τ) τ = true 
+decreasing τ₁ τ₂ =  
+  any τ₁ (.l τ => decreasing τ (project τ₂ l)) andalso
+  all τ₁ (.l τ => ¬ increasing τ (project τ₂ l))
+```
+
+`increasing τ τ = b`
+```
+increasing τ₁ τ₂ = decreasing τ₂ τ₁
+```
+
+`well_founded α τ = b`
+```
+well_founded α τ₁ | τ₂ = 
+  cases_normal τ₁ τ₂ andalso
+  well_founded α τ₁ andalso
+  well_founded α τ₂
+
+well_founded α ∀ Δ ⟨τ' ≤ α⟩ . τ = 
+  α ∈ Δ orelse
+  decreasing τ τ' 
+```
+-/
+
+/-
+
+`occurs α τ`
+```
+occurs α α = true
+occurs α ? = false 
+occurs α ⟨⟩ = false 
+occurs α (#l τ) = occurs α τ 
+occurs α (.l τ) = occurs α τ 
+occurs α (τ₁ -> τ₂) = (occurs α τ₁) orelse (occurs α τ₂)
+occurs α (τ₁ & τ₂) = (occurs α τ₁) orelse (occurs α τ₂)
+occurs α (τ₁ | τ₂) = (occurs α τ₁) orelse (occurs α τ₂)
+occurs α (∀ Δ ⟨C⟩ . τ) = 
+  α ∉ Δ andalso
+  (occurs α C) orelse (occurs α τ)
+occurs α (μ β . t) = 
+  α ≠ β andalso 
+  (occurs α τ)
+```
+
+`occurs α C`
+```
+occurs α (τ' ≤ τ) = (occurs α τ') orelse (occurs α τ)
+occurs α (C₁ ∨ C₂) = (occurs α C₁) orelse (occurs α C₂)
+occurs α (C₁ ∧ C₂) = (occurs α C₁) orelse (occurs α C₂)
+```
+-/
+
+-- occurs: check if free variable exists in type
+mutual
+  partial def Ty.occurs (key : Nat)  : Ty -> Bool 
+    | [: ? :] => false 
+    | .bvar id => false 
+    | .fvar id => key = id 
+    | .unit => false 
+    | .variant l ty => (Ty.occurs key ty) 
+    | .field l ty => (Ty.occurs key ty)
+    | [: ⟨ty₁⟩ | ⟨ty₂⟩ :] => (Ty.occurs key ty₁) ∨ (Ty.occurs key ty₂)
+    -- | .union ty₁ ty₂ => (Ty.occurs key ty₁) ∨ (Ty.occurs key ty₂)
+    | .inter ty₁ ty₂ => (Ty.occurs key ty₁) ∨ (Ty.occurs key ty₂)
+    | .func ty₁ ty₂ => (Ty.occurs key ty₁) ∨ (Ty.occurs key ty₂)
+    | .univ ctx c ty => (
+      (List.any ctx (λ cty => Ty.occurs key cty)) ∨
+      (Constr.occurs key c) ∨
+      (Ty.occurs key ty)
+    )
+    | .induct ty => (Ty.occurs key ty)
+
+  partial def Constr.occurs (key : Nat) : Constr -> Bool
+    | Constr.tru => false 
+    | Constr.subtype ty₁ ty₂ => (Ty.occurs key ty₁) ∨ (Ty.occurs key ty₂)
+    | Constr.conj c₁ c₂ => (Constr.occurs key c₁) ∨ (Constr.occurs key c₂)
+    | Constr.disj c₁ c₂ => (Constr.occurs key c₁) ∨ (Constr.occurs key c₂)
+end
+
+mutual
+  partial def Ty.eq : Ty -> Ty -> Bool 
+    | .unknown, .unknown => true 
+    | .bvar id1, .bvar id2 => id1 = id2 
+    | .fvar id1, .fvar id2 => id1 = id2 
+    | .unit, .unit => true 
+    | .variant l1 ty1, .variant l2 ty2 => 
+      l1 = l2 ∧ (Ty.eq ty1 ty2) 
+    | .field l1 ty1, .field l2 ty2 =>
+      l1 = l2 ∧ (Ty.eq ty1 ty2) 
+    | .union ty₁ ty₂, .union ty₃ ty₄ => 
+      (Ty.eq ty₁ ty₃) ∧ (Ty.eq ty₂ ty₄)
+    | .inter ty₁ ty₂, .inter ty₃ ty₄ => 
+      (Ty.eq ty₁ ty₃) ∧ (Ty.eq ty₂ ty₄)
+    | .func ty₁ ty₂, .func ty₃ ty₄  => 
+      (Ty.eq ty₁ ty₃) ∧ (Ty.eq ty₂ ty₄)
+    | .univ ctx₁ c₁ ty₁, .univ ctx₂ c₂ ty₂ =>
+      (List.isEqv ctx₁ ctx₂ (fun cty₁ cty₂ => Ty.eq cty₁ cty₂)) ∧
+      (Constr.eq c₁ c₂) ∧ (Ty.eq ty₁ ty₂)
+    | .induct ty₁, .induct ty₂ => (Ty.eq ty₁ ty₂)
+    | _, _ => false
+
+  partial def Constr.eq : Constr -> Constr -> Bool
+    | Constr.tru, Constr.tru => true 
+    | Constr.subtype ty₁ ty₂, Constr.subtype ty₃ ty₄ => 
+      (Ty.eq ty₁ ty₃) ∧ (Ty.eq ty₂ ty₄)
+    | Constr.conj c₁ c₂, Constr.conj c₃ c₄ =>
+      (Constr.eq c₁ c₃) ∧ (Constr.eq c₂ c₄)
+    | Constr.disj c₁ c₂, Constr.disj c₃ c₄ =>
+      (Constr.eq c₁ c₃) ∧ (Constr.eq c₂ c₄)
+    | _, _ => false
+end
+
+
+
+
+mutual
+
+
+  partial def Ty.free_subst (m : List (Nat × Ty)) : Ty -> Ty
+    | .unknown => .unknown 
+    | .bvar id => .bvar id 
+    | .fvar id => (match lookup id m with
+      | some ty => ty 
+      | none => .fvar id
+    )
+    | .unit => .unit
+    | .variant l ty => .variant l (Ty.free_subst m ty) 
+    | .field l ty => .field l (Ty.free_subst m ty)
+    | .union ty₁ ty₂ => .union (Ty.free_subst m ty₁) (Ty.free_subst m ty₂)
+    | .inter ty₁ ty₂ => .inter (Ty.free_subst m ty₁) (Ty.free_subst m ty₂)
+    | .func ty₁ ty₂ => .func (Ty.free_subst m ty₁) (Ty.free_subst m ty₂)
+    | .univ ctx c ty => (.univ
+      (List.map (λ cty => Ty.free_subst m cty) ctx) 
+      (Constr.free_subst m c) 
+      (Ty.free_subst m ty)
+    )
+    | .induct ty => .induct (Ty.free_subst m ty)
+
+  partial def Constr.free_subst (m : List (Nat × Ty)) : Constr -> Constr
+    | Constr.tru => Constr.tru
+    | Constr.subtype ty₁ ty₂ => Constr.subtype (Ty.free_subst m ty₁) (Ty.free_subst m ty₂)
+    | Constr.conj c₁ c₂ => Constr.conj (Constr.free_subst m c₁) (Constr.free_subst m c₂)
+    | Constr.disj c₁ c₂ => Constr.disj (Constr.free_subst m c₁) (Constr.free_subst m c₂)
+end
+
+
+declare_syntax_cat sub
+syntax slm "/" slm : sub 
+syntax "[" sub,+ "]" : sub
+syntax "[sub:" sub ":]" : term 
+
+macro_rules
+  | `([sub: $a:slm / $b:slm :]) => `(([: $a :], [: $b :])) 
+
+macro_rules
+  | `([sub: [$x:sub] :]) => `([ [sub: $x :] ])
+  | `([sub: [$x,$xs:sub,*] :]) => `([sub: $x :] :: [sub: [$xs,*] :])
+
+
+syntax slm "%" sub : slm 
+macro_rules
+  | `([: $a % $b:sub :]) => `(Ty.free_subst [sub: $b :] [: $a :])
+
+
+-- #check [: (£1) % [1 / ?] :]
+#check [: (£1) % [1/?] :]
+
+#check Fin
+
+mutual
+  partial def Ty.raise_binding (start : Nat) (args : List Ty) : Ty -> Ty
+    | .unknown => .unknown 
+    | .bvar id => 
+        if h : start ≤ id ∧ (id - start) < args.length then
+          let i : Fin args.length := {
+            val := (id - start),
+            isLt := (match h with | And.intro _ h' => h') 
+          } 
+          args.get i 
+        else
+          .bvar id
+    | .fvar id => .fvar id 
+    | .unit => .unit
+    | .variant l ty => .variant l (Ty.raise_binding start args ty) 
+    | .field l ty => .field l (Ty.raise_binding start args ty)
+    | .union ty₁ ty₂ => .union (Ty.raise_binding start args ty₁) (Ty.raise_binding start args ty₂)
+    | .inter ty₁ ty₂ => .inter (Ty.raise_binding start args ty₁) (Ty.raise_binding start args ty₂)
+    | .func ty₁ ty₂ => .func (Ty.raise_binding start args ty₁) (Ty.raise_binding start args ty₂)
+    | .univ ctx c ty => (.univ
+      (List.map (λ cty => Ty.raise_binding (start + ctx.length) args cty) ctx) 
+      (Constr.raise_binding (start + ctx.length) args c) 
+      (Ty.raise_binding (start + ctx.length) args ty)
+    )
+    | .induct ty => .induct (Ty.raise_binding (start + 1) args ty)
+
+  partial def Constr.raise_binding (start : Nat) (args : List Ty) : Constr -> Constr
+    | .tru => .tru 
+    | .subtype ty₁ ty₂ => .subtype (Ty.raise_binding start args ty₁) (Ty.raise_binding start args ty₂)
+    | .conj c₁ c₂ => .conj (Constr.raise_binding start args c₁) (Constr.raise_binding start args c₂)
+    | .disj c₁ c₂ => .disj (Constr.raise_binding start args c₁) (Constr.raise_binding start args c₂)
+end
+
+syntax slm "↑" slm "/" slm : slm 
+
+macro_rules
+  | `([: $a ↑ $b / $c :]) => `(Ty.raise_binding [: $b :] [: $c :] [: $a :])
+
+
+def τ := [: ? :]
+#check [: ⟨τ⟩ ↑ 0 / [μ 0 . ⟨τ⟩]:]
+
+-- termination_by 
+--   Ty.subst _ ty => (some ty, none)
+--   Constr.subst _ c => (none, some c)
+-- decreasing_by sorry
+
+
+/-
+`unroll μ α . τ = τ`
+```
+unroll μ α . τ = subst {α ≤ μ α . τ} τ
+```
+-/
+partial def unroll (τ : Ty) : Ty := 
+  -- Ty.raise_binding 0 [Ty.induct τ] τ 
+  [: ⟨τ⟩ ↑ 0 / [μ 0 . ⟨τ⟩]:]
+
+/-
+
+`rename m Δ`
+```
+rename m Δ = 
+  map Δ (α / τ =>
+    let β = m α in
+    {β / subst m τ}
+  )
+```
+-/
+
+
+/-
+`roll α τ`
+```
+roll α τ = 
+  μ α . τ
+  if occurs α τ else
+  τ
+```
+-/
+
+mutual
+  partial def Ty.lower_binding (depth : Nat) : Ty -> Ty
+    | .unknown => .unknown 
+    | .bvar id => .bvar (id + depth)
+    | .fvar id => .fvar id 
+    | .unit => .unit
+    | .variant l ty => .variant l (Ty.lower_binding depth ty) 
+    | .field l ty => .field l (Ty.lower_binding depth ty)
+    | .union ty₁ ty₂ => .union (Ty.lower_binding depth ty₁) (Ty.lower_binding depth ty₂)
+    | .inter ty₁ ty₂ => .inter (Ty.lower_binding depth ty₁) (Ty.lower_binding depth ty₂)
+    | .func ty₁ ty₂ => .func (Ty.lower_binding depth ty₁) (Ty.lower_binding depth ty₂)
+    | .univ ctx c ty => (.univ
+      (List.map (λ cty => Ty.lower_binding (depth + ctx.length) cty) ctx) 
+      (Constr.lower_binding (depth + ctx.length) c) 
+      (Ty.lower_binding (depth + ctx.length) ty)
+    )
+    | .induct ty => .induct (Ty.lower_binding (depth + 1) ty)
+
+  partial def Constr.lower_binding (depth : Nat) : Constr -> Constr
+    | Constr.tru => Constr.tru
+    | Constr.subtype ty₁ ty₂ => Constr.subtype (Ty.lower_binding depth ty₁) (Ty.lower_binding depth ty₂)
+    | Constr.conj c₁ c₂ => Constr.conj (Constr.lower_binding depth c₁) (Constr.lower_binding depth c₂)
+    | Constr.disj c₁ c₂ => Constr.disj (Constr.lower_binding depth c₁) (Constr.lower_binding depth c₂)
+end
+
+syntax slm "↓" num : slm 
+
+macro_rules
+  | `([: $b:slm ↓ $a:num :]) => `(Ty.lower_binding $a [: $b :])
+
+
+partial def roll (key : Nat) (τ : Ty) : Ty :=
+  if Ty.occurs key τ then
+    [: (μ 0 . ⟨τ⟩↓1) % [⟨key⟩ / £0] :]
+  else
+    τ
+
+
+
+/-
+`Δ α = τ` 
+```
+Δ α =  
+  τ
+  if {α → τ} ⊆ Δ else
+  ?
+```
+
+-/
+
+
+def liberate (i : Nat) : List Ty -> List (Nat × Ty) 
+  | [] => []
+  | cty :: ctx => (i, cty) :: (liberate (i + 1) ctx)
+
+def refresh (i : Nat) (ctx : List Ty) : (Nat × List (Nat × Ty) × List Ty) := 
+  let args := (List.range ctx.length).map (fun j => .fvar (i + j))
+  let f : Ty -> Ty := Ty.raise_binding 0 args 
+  let Δ' := liberate i (ctx.map f)
+  let i' := i + ctx.length
+  (i', Δ', args)
+
+
+def make_record_constraint_sub (prev_ty : Ty) : Ty -> Ty -> Option Constr
+  | (.field l ty'), mu_ty => 
+      let ty := .univ [Ty.unknown] (Constr.subtype 
+        (Ty.inter (Ty.lower_binding 1 prev_ty) (.field l (.bvar 0))) (Ty.lower_binding 1 (unroll mu_ty))
+      ) (.bvar 0)
+      some (Constr.subtype ty' ty)
+  | .inter (.field l ty') rem_ty, mu_ty => 
+      let ty := 
+      [: ∀ [?] ((⟨prev_ty⟩↓1 & (#⟨l⟩ £0) & ⟨rem_ty⟩↓1) ≤ ⟨unroll mu_ty⟩↓1) . £0 :]
+
+      Option.bind (
+        make_record_constraint_sub (Ty.inter prev_ty (.field l ty')) rem_ty mu_ty
+      ) (fun rem =>
+        some (Constr.conj (Constr.subtype ty' ty) rem
+      ))
+  | .inter rem_ty (.field l ty'), mu_ty => 
+      -- copy and paste above case (for terminateion proved by structure)
+      let ty := .univ [Ty.unknown] (Constr.subtype 
+        (Ty.inter (
+          Ty.inter (Ty.lower_binding 1 prev_ty) (.field l (.bvar 0))) 
+          (Ty.lower_binding 1 rem_ty)
+        ) (Ty.lower_binding 1 (unroll mu_ty))
+      ) (.bvar 0)
+
+      Option.bind (
+        make_record_constraint_sub (Ty.inter prev_ty (.field l ty')) rem_ty mu_ty
+      ) (fun rem =>
+        some (Constr.conj (Constr.subtype ty' ty) rem
+      ))
+  | _, _ =>  none
+
+def make_record_constraint_super (prev : Ty) : Ty -> Ty -> Option Constr
+  | mu_ty, (.field l ty') => 
+      let ty := .univ [Ty.unknown] (Constr.subtype 
+        (Ty.lower_binding 1 (unroll mu_ty))
+        (Ty.inter (Ty.lower_binding 1 prev) (.field l (.bvar 0))) 
+      ) (.bvar 0)
+      some (Constr.subtype ty' ty)
+  | mu_ty, .inter (.field l ty') rem_ty => 
+      let ty := .univ [Ty.unknown] (Constr.subtype 
+        (Ty.lower_binding 1 (unroll mu_ty))
+        (Ty.inter (
+          Ty.inter (Ty.lower_binding 1 prev) (.field l (.bvar 0))) 
+          (Ty.lower_binding 1 rem_ty)
+        ) 
+      ) (.bvar 0)
+
+      Option.bind (
+        make_record_constraint_super (Ty.inter prev (.field l ty')) mu_ty rem_ty
+      ) (fun rem =>
+        some (Constr.conj (Constr.subtype ty' ty) rem
+      ))
+  | mu_ty, .inter rem_ty (.field l ty') => 
+      -- copy and paste above case (for terminateion proved by structure)
+      let ty := .univ [Ty.unknown] (Constr.subtype 
+        (Ty.lower_binding 1 (unroll mu_ty))
+        (Ty.inter (
+          Ty.inter (Ty.lower_binding 1 prev) (.field l (.bvar 0))) 
+          (Ty.lower_binding 1 rem_ty)
+        ) 
+      ) (.bvar 0)
+
+      Option.bind (
+        make_record_constraint_super (Ty.inter prev (.field l ty')) mu_ty rem_ty
+      ) (fun rem =>
+        some (Constr.conj (Constr.subtype ty' ty) rem
+      ))
+  | _, _ =>  none
+
+
+mutual
+  partial def Ty.unify (i : Nat) (Δ : List (Nat × Ty)) : Ty -> Ty -> Option (Nat × List (Nat × Ty))
+
+    | .fvar id, τ₂  => match lookup id Δ with 
+      | none => some (i + 2, [(i, .inter (roll id τ₂) (Ty.fvar (i + 1)))]) 
+      | some Ty.unknown => some (i + 2, [(i, .inter (roll id τ₂) (Ty.fvar (i + 1)))]) 
+      | some τ₁ => Ty.unify i Δ τ₁ τ₂ 
+
+    | τ₁, .fvar id  => match lookup id Δ with 
+      | none => some (i + 2, [(i, .union (roll id τ₁) (Ty.fvar (i + 1)))]) 
+      | some Ty.unknown => some (i + 2, [(i, .union (roll id τ₁) (Ty.fvar (i + 1)))]) 
+      | some τ₂ => Ty.unify i Δ τ₁ τ₂ 
+
+    | .induct τ', .induct τ =>
+      Ty.unify i Δ τ' τ 
+
+    | .variant l' τ', .induct τ =>
+      Ty.unify i Δ (.variant l' τ') (unroll τ)
+
+    | .induct τ', (.variant l τ) =>
+      Ty.unify i Δ (unroll τ') (.variant l τ) 
+
+    | τ', .induct τ =>
+      Option.bind (make_record_constraint_sub Ty.unknown τ' τ) (fun c =>
+        Constr.solve i Δ c
+      )
+
+    | .induct τ', τ =>
+      Option.bind (make_record_constraint_super Ty.unknown τ' τ) (fun c =>
+        Constr.solve i Δ c
+      )
+
+    | .union τ₁ τ₂, τ => 
+      Constr.solve i Δ (Constr.conj 
+        (Constr.subtype τ₁ τ)
+        (Constr.subtype τ₂ τ)
+      )
+
+    | τ, .union τ₁ τ₂ => 
+      Constr.solve i Δ (Constr.disj 
+        (Constr.subtype τ τ₁)
+        (Constr.subtype τ τ₂)
+      )
+
+    | τ, .inter τ₁ τ₂ => 
+      Constr.solve i Δ (Constr.conj
+        (Constr.subtype τ τ₁)
+        (Constr.subtype τ τ₂)
+      )
+
+    | .inter τ₁ τ₂, τ => 
+      Constr.solve i Δ (Constr.disj
+        (Constr.subtype τ₁ τ)
+        (Constr.subtype τ₂ τ)
+      )
+
+    | .func τ₁ τ₂', .func τ₁' τ₂ =>
+      Constr.solve i Δ (Constr.conj
+        (Constr.subtype τ₁' τ₁)
+        (Constr.subtype τ₂' τ₂)
+      )
+
+    | .variant l' τ', .variant l τ =>
+      if l' = l then
+        Ty.unify i Δ τ' τ
+      else
+        none
+
+    | .field l' τ', .field l τ =>
+      if l' = l then
+        Ty.unify i Δ τ' τ
+      else
+        none
+
+    | ty, .univ ctx c τ =>
+      let (i, Δ, args) := refresh i ctx
+      let c := Constr.raise_binding 0 args c
+      let τ := Ty.raise_binding 0 args τ
+      Constr.solve i Δ (Constr.conj c (Constr.subtype ty τ))
+
+    | .univ ctx c τ, ty =>
+      let (i, Δ, args) := refresh i ctx
+      let c := Constr.raise_binding 0 args c
+      let τ := Ty.raise_binding 0 args τ
+      Constr.solve i Δ (Constr.conj c (Constr.subtype τ ty))
+
+    | .bvar id₁, .bvar id₂  =>
+      if id₁ = id₂ then 
+        some (i, [])
+      else
+        none
+
+    | .unit, .unit => some (i, []) 
+    | .unknown, _ => some (i, []) 
+    | _, .unknown => some (i, []) 
+    | _, _ => none
+
+  partial def Constr.solve (i : Nat) (Δ : List (Nat × Ty)) : Constr -> Option (Nat × List (Nat × Ty))
+    | Constr.tru => some (i, []) 
+    | Constr.subtype ty₁ ty₂ => Ty.unify i Δ ty₁ ty₂
+    | Constr.conj c₁ c₂ => 
+        Option.bind (Constr.solve i Δ c₁) (fun (i, Δ₁) => 
+        Option.bind (Constr.solve i Δ c₂) (fun (i, Δ₂) =>
+          some (i, merge Ty.inter Ty.unknown Δ₁ Δ₂)
+        ))
+    | Constr.disj c₁ c₂ =>
+        Option.bind (Constr.solve i Δ c₁) (fun (i, Δ₁) => 
+        Option.bind (Constr.solve i Δ c₂) (fun (i, Δ₂) =>
+          some (i, merge Ty.union Ty.unknown Δ₁ Δ₂)
+        ))
+end
+
+/-
+
+`solve Δ ⊢ C = o[Δ]`
+```
+solve Δ ⊢ C₁ ∧ C₂ =  
+  merge & (solve Δ ⊢ C₁) (solve Δ ⊢ C₂)
+
+solve Δ ⊢ C₁ ∨ C₂ = 
+  merge | (solve Δ ⊢ C₁) (solve Δ ⊢ C₂)
+
+solve Δ ⊢ α ≤ τ =
+  let τ' = Δ α in (
+    let β = fresh in some {α ≤ ((roll α τ) & β), β ≤ ?}
+    if τ' = ? else
+    solve Δ ⊢ τ' ≤ τ
+  )
+
+solve Δ ⊢ τ' ≤ α =
+  let τ = Δ α in (
+    let β = fresh in some {α ≤ ((roll α τ') | β), β ≤ ?}  
+    if τ = ? else
+    (solve Δ ⊢ τ' ≤ τ)
+  )
+
+solve Δ ⊢ (∀ Δ' ⟨C⟩ . τ') ≤ τ =
+...
+
+solve Δ ⊢ τ' ≤ (∀ Δ' ⟨C⟩ . τ) =
+...
+
+solve Δ ⊢ τ₁ | τ₂ ≤ τ =
+  solve Δ ⊢ τ₁ ≤ τ ∧ τ₂ ≤ τ
+
+solve Δ ⊢ τ ≤ τ₁ | τ₂ =
+  solve Δ ⊢ τ ≤ τ₁ ∨ τ ≤ τ₂
+
+
+solve Δ ⊢ τ ≤ τ₁ & τ₂ =
+  solve Δ ⊢ τ ≤ τ₁ ∧ τ ≤ τ₂
+
+solve Δ ⊢ τ₁ & τ₂ ≤ τ =
+  solve Δ ⊢ τ₁ ≤ τ ∨ τ₂ ≤ τ
+
+solve Δ ⊢ τ₁ -> τ₂' ≤ τ₁' -> τ₂ =
+  solve Δ ⊢ τ₁' ≤ τ₁ ∧ τ₂' ≤ τ₂
+
+
+solve Δ ⊢ #l τ' ≤ μ α . τ =  
+  solve Δ ⊢ #l τ' ≤ unroll (μ α . τ)  
+
+solve Δ ⊢ μ α . τ' ≤ #l τ  =  
+  solve Δ ⊢ unroll (μ α . τ') ≤ #l τ
+
+solve Δ ⊢ .l τ' ≤ μ α . τ =  
+  solve Δ ⊢ .l τ' ≤ unroll (μ α . τ)  
+
+solve Δ ⊢ μ α . τ' ≤ .l τ  =  
+  solve Δ ⊢ unroll (μ α . τ') ≤ .l τ
+
+
+solve Δ ⊢ τ' ≤ μ α . τ =
+  map (linearze_record τ') (τ' =>
+  map (make_record_constraint Δ ⊢ . * τ' ≤ μ α . τ) (C =>
+    solve Δ ⊢ C 
+  ))
+
+solve Δ ⊢ μ α . τ' ≤ τ  =  
+  map (linearze_record τ') (τ' =>
+  map (make_record_constraint Δ ⊢ . * μ α . τ' ≤ τ) (C =>
+    solve Δ ⊢ C 
+  ))
+
+solve Δ ⊢ #l' τ' ≤ #l τ =
+  solve Δ ⊢ τ' ≤ τ
+  if l' = l else
+  none
+
+solve τ ≤ τ = some {} 
+solve _ = none 
+```
+
+`patvars t = o[Γ]`
+```
+patvars x τ = 
+  some {x : τ}
+patvars (.l t₁) τ = 
+  map (project τ l) (τ₁ =>
+    patvars t₁ τ₁
+  )
+patvars (.l t fs) τ =
+  map (patvars (.l t) τ) (Γ₁ =>
+  map (patvars fs τ) (Γ₂ =>
+    some (Γ₁ ++ Γ₂)
+  ))
+...
+```
+
+
+`infer Γ Δ ⊢ t : τ = o[Δ;τ]`
+```
+TODO:
+- raise type binding at application in "infer/generation of constrations"
+
+infer Γ Δ ⊢ () : τ =
+  map (solve Δ ⊢ C ∧ [] ≤ τ in) (Δ' =>
+    some (Δ' , [])
+  )
+
+infer Γ Δ ⊢ x : τ = 
+  let τ' = Γ x in
+  let Δ', C, τ' = refresh τ' in
+  map (solve Δ, Δ' ⊢ C ∧ τ' ≤ τ) (Δ' =>
+    some (Δ' , τ')
+  )
+
+infer Γ Δ ⊢ (#l t₁) : τ =
+  let α = fresh in
+  map (solve Δ ⊢ (∀ {α} . (#l α)) ≤ τ) (Δ' => 
+  map (infer Γ (Δ ++ Δ') ⊢ t₁ : α) (Δ₁,τ₁ => 
+    some (Δ' ++ Δ₁ , #l τ₁)
+  ))
+
+infer Γ Δ ⊢ (for t₁ : τ₁ => t₂) : τ =
+  let Δ₁, τ₁ = τ₁[?/fresh] in
+  let Γ₁ = patvars t₁ τ₁ in
+  let β = fresh in
+  map (solve Δ ⊢ (∀ Δ₁ ++ {β} . τ₁ -> β) ≤ τ) (Δ' => 
+  map (infer (Γ ++ Γ₁) (Δ ++ Δ') ⊢ t₂ : β) (Δ₂', τ₂' =>
+    -- patvars (Γ₁) are NOT generalized in τ₂'
+    some (Δ' ++ Δ₂' , τ₁ -> τ₂')
+  ))
+
+
+infer Γ Δ ⊢ (for t₁ : τ₁ => t₂) cs : τ =
+  map (infer Γ Δ ⊢ (for t₁ : τ₁ => t₂) : τ) (Δ', τ' =>
+  map (infer Γ Δ ++ Δ' ⊢ cs : τ₂) (Δ'', τ'' => 
+    some (Δ' ++ Δ'' , τ' & τ'')
+  ))
+
+infer Γ Δ ⊢ t t₁ : τ₂ =
+  map (infer Γ Δ ⊢ t : ? -> τ₂ in) (Δ',τ' => 
+  map (functify τ') (τ₁,τ₂' => 
+  -- break type (possibly intersection) into premise and conclusion 
+  map (infer Γ (Δ ++ Δ') ⊢ t₁ : τ₁) (Δ₁',τ₁' =>
+  map (solve Δ ++ Δ' ++ Δ₁' ⊢ τ' ≤ (τ₁' -> τ₂)) (Δ' =>
+    some(Δ' , τ₂' & τ₂)
+  ))))
+
+infer Γ Δ ⊢ (.l t₁) : τ =
+  let α = fresh in
+  map (solve Δ ⊢ (∀ {α} . (.l α)) ≤ τ) (Δ' =>
+  map (infer Γ (Δ ++ Δ') ⊢ t₁ : α) (Δ₁ , τ₁ =>  
+    some(Δ' ++ Δ₁ , .l τ₁)
+  ))
+
+infer Γ Δ ⊢ (.l t₁) fs : τ =
+  map (infer Γ Δ ⊢ (.l t₁) : τ) (Δ' , τ' =>
+  map (infer Γ (Δ ++ Δ') ⊢ fs : τ) (Δ'' , τ'' =>
+    some(Δ' ++ Δ'' , τ' & τ'')
+  ))
+
+infer Γ Δ ⊢ t.l : τ₂ =
+  map (infer Γ Δ ⊢ t : (.l τ₂)) (Δ' , τ' =>
+  map (project τ' l) (τ₂' => 
+    some(Δ' , τ₂')
+  ))
+
+infer Γ Δ ⊢ fix t : τ =
+  map (infer Γ Δ ⊢ t : (τ -> τ)) (Δ',τ' =>
+  map (functify τ') (τ₁', τ₂' =>
+    -- extract premise and conclusion 
+    some(Δ' , τ₂')
+  ))
+
+infer Γ Δ ⊢ (let x : τ₁ = t₁ in t₂) : τ₂ =
+  let Δ₁,τ₁ = τ₁[?/fresh] in
+  map (infer Γ Δ ⊢ t₁ : (∀ Δ₁ . τ₁)) (Δ₁' , τ₁' => 
+  map (infer (Γ ++ {x : (∀ Δ₁' . τ₁')}) Δ ⊢ t₂ : τ₂) (Δ₂' , τ₂' =>
+    -- τ₁' is generalized in τ₂'
+    some(Δ₂' , τ₂')
+  ))
+```
+
+-/
+
+-- static implementation/semantics theorems
+/-
+soundness: ...
+completeness: ...
+-/
+
+
+-- static/dynamic semantics theorems
+/-
+soundness: N/A
+completeness: N/A
 -/
 
 
@@ -247,579 +1493,3 @@ let hello' = f hello in
 ))
 ```
 -/
-
--- syntax 
-/-
-
-x ∈ String                        term variable
-l ∈ String                        label
-
-cs ::=                            cases
-  for t => t                      case singleton 
-  for t => t cs                   cases extended 
-
-fs ::=                            fields 
-  .l t                            field singleton 
-  .l t fs                         fields extended 
-
-t ::=                             term
-  __                              hole / irrelevant pattern
-  x                               variable expression / pattern
-  ()                              unit expression / pattern
-  #l t                            variant expression / pattern
-  fs                              record expression / pattern
-  t.l                             record projection
-  cs                              function expression
-  t t                             function application
-  let t : τ = t in t              binding
-  fix t                           recursion
-
-α ∈ String                        type variable
-
-τ ::=                             type
-  α                               variable type
-  ?                               unknown type
-  []                              unit type
-  #l τ                            variant type
-  .l τ                            field type
-  τ -> τ                          implication type 
-  τ & τ                           intersection type
-  τ | τ                           union type
-  ∀ Δ C τ                         universal schema 
-  μ α . τ                         inductive type
-  [τ]                             grouped type
-
-C ::=                             constraint
-  .                               true
-  ⟨C⟩                             grouped constraint 
-  τ ≤ τ                           subtyping 
-  C ∨ C                           disjunction
-  C ∧ C                           conjunction
-
-Δ ::=                             type context
-  {..., α ≤ τ, ...}
-  Δ ∪ Δ                        
-
-m ::=                             substitution 
-  {..., α / τ, ...}
-  m ∪ m                        
-
-o[i] ::= some[i] | none           option
-
-Γ ::=                             term context
-  {..., x : τ, ...}                        
-  Γ ∪ Γ                      
-
--/
-
--- dynamic semantics 
-/-
--/
-
--- dynamic implementation 
-/-
-beyond scope
--/
-
--- dynamic semantics/implementation theorems
-/-
-beyond scope
--/
-
--- static semantics 
-/-
-
-consistent constraint subtyping   
-`Δ ⊢ C`
-```
-Δ ⊢ .
-
-  Δ ⊢ C 
----
-Δ ⊢ ⟨C⟩ 
-
-  Δ ⊢ C₁ 
-  Δ ⊢ C₂
----
-Δ ⊢ C₁ ∧ C₂ 
-
-  Δ ⊢ C₁ 
----
-Δ ⊢ C₁ ∨ C₂ 
-
-  Δ ⊢ C₂
----
-Δ ⊢ C₁ ∨ C₂ 
-
-Δ ⊢ τ ≤ τ
-
-Δ ⊢ τ ≤ ? 
-
-Δ ⊢ ? ≤ τ 
-
-  Γ ⊢ τ' ≤ τₘ
-  Γ ⊢ τₘ ≤ τ
-  τₘ ≠ ?
----
-Δ ⊢ τ' ≤ τ  
-
-
-  {α ≤ τ} ⊆ Δ
----
-Δ ⊢ α ≤ τ  
-
-
-  Δ₀, Δ' ⊢ C' ∧ τ' ≤ τ
----
-Δ₀ ⊢ (∀ Δ' C' τ') ≤ τ
-
-
-  Δ₀, Δ ⊢ C ∧ τ' ≤ τ
----
-Δ₀ ⊢ τ' ≤ (∀ Δ C τ)
-
-
-Δ₀ ⊢ (μ α . τ) ≤ unroll (μ α . τ)
-
-
-Δ₀ ⊢ unroll (μ α . τ) ≤ (μ α . τ)
-
-
-  Δ ⊢ τ₁' ≤ τ₁ 
-  Δ ⊢ τ₂' ≤ τ₂ 
----
-Δ ⊢ τ₁ -> τ₂' ≤ τ₁' -> τ₂
-
-
-  Δ ⊢ τ' ≤ τ
----
-Δ ⊢ .l τ' ≤ .l τ  
-
-
-  Δ ⊢ τ' ≤ τ  
----
-Δ ⊢ #l τ' ≤ #l τ
-
-
-Δ ⊢ τ' ≤ (τ' | τ)  
-
-Δ ⊢ τ' ≤ (τ | τ')  
-
-
-  Δ ⊢ τ₁ ≤ τ   
-  Δ ⊢ τ₂ ≤ τ  
----
-Δ ⊢ (τ₁ | τ₂) ≤ τ 
-
-
-Δ ⊢ (τ & τ') ≤ τ
-
-Δ ⊢ (τ' & τ) ≤ τ  
-
-
-  Δ ⊢ τ' ≤ τ₁  
-  Δ ⊢ τ' ≤ τ₂  
----
-Δ ⊢ τ' ≤ τ₁ & τ₂  
-```
-
-constraint typing  
-`Γ Δ C ⊢ t : τ`
-```
-TODO: fill in constraint typing rules
-```
-
--/
-
--- static implementation 
-/-
-
-
-`merge Δ Δ = Δ`
-```
-merge op Δ₁ Δ₂ =
-  fmap Δ₁ (α ≤ τ₁ =>
-  fmap Δ₂ (β ≤ τ₂ =>
-    {α ≤ τ₁ op (Δ₂ α), β ≤ (Δ₁ β) op τ₂}
-  ))
-```
-
-`merge o[Δ] o[Δ] = o[Δ]`
-```
-merge _ none none = none 
-merge _ none o = o 
-merge _ o none = o 
-merge op (some Δ₁) (some Δ₂) = some (merge op Δ₁ Δ₂)
-```
-
-
-`linearize_record τ = o[fs]`
-```
-linearize_record .l₁ τ₁ & .l₂ τ₂ =
-  some (.l₁ τ₁ & .l₂ τ₂)
-linearize_record .l τ₁ & τ₂ =
-  some .l τ₁ & (linearize_record τ₂)
-linearize_record τ₁ & .l τ₂ =
-  some .l τ₂ & (linearize_record τ₁)
-linearize_record τ₁ & τ₂ =
-  none
-```
-
-`make_field_constraint Δ ⊢ τ * τ ≤ τ = o[C]`
-```
-make_field_constraint Δ ⊢ τ₀ * .l τ₁ & τ₂ ≤ μ α . τ =
-  let β₁ = fresh in
-  let C₁ = τ₁ ≤ ∀ {β₁ ≤ ?} ⟨(τ₀ & .l β₁ & τ₂) ≤ unroll (μ α . τ)⟩ . β₁ in
-  C₁ ∧ make_field_constraint (Δ ⊢ τ₀ & .l τ₁ * τ₂ ≤ μ α . τ)
-
-make_field_constraint Δ ⊢ τ₀ * .l τ₁ ≤ μ α . τ =
-  let β₁ = fresh in
-  let C₁ = τ₁ ≤ ∀ {β₁ ≤ ?} ⟨(τ₀ & .l β₁) ≤ unroll (μ α . τ)⟩ . β₁ in
-  C₁
-
-make_field_constraint _ ⊢ _ * _ ≤ _ = none
-```
-
-`match o o = b`
-```
-match (some x₁) (some ×₂) = 
-  x₁ = x₂
-match none _ = false
-match _ none = false
-```
-
-`cases_normal τ τ = b`
-```
-cases_normal (#l₁ τ₁) (#l₂ τ₂) = true
-cases_normal τ₁ τ₂ = 
-  fmap (keys τ₁) (ks₁ =>
-  fmap (keys τ₂) (ks₂ =>
-    some (ks₁ = ks₂)
-  )) = Some true
-  (keys τ₁) = (keys τ₂) 
-```
-
-
-`decreasing τ τ = b`
-```
-decreasing (#l τ) τ = true 
-decreasing τ₁ τ₂ =  
-  any τ₁ (.l τ => decreasing τ (project τ₂ l)) andalso
-  all τ₁ (.l τ => ¬ increasing τ (project τ₂ l))
-```
-
-`increasing τ τ = b`
-```
-increasing τ₁ τ₂ = decreasing τ₂ τ₁
-```
-
-`well_founded α τ = b`
-```
-well_founded α τ₁ | τ₂ = 
-  cases_normal τ₁ τ₂ andalso
-  well_founded α τ₁ andalso
-  well_founded α τ₂
-
-well_founded α ∀ Δ ⟨τ' ≤ α⟩ . τ = 
-  α ∈ Δ orelse
-  decreasing τ τ' 
-```
-
-`occurs α τ`
-```
-occurs α α = true
-occurs α ? = false 
-occurs α ⟨⟩ = false 
-occurs α (#l τ) = occurs α τ 
-occurs α (.l τ) = occurs α τ 
-occurs α (τ₁ -> τ₂) = (occurs α τ₁) orelse (occurs α τ₂)
-occurs α (τ₁ & τ₂) = (occurs α τ₁) orelse (occurs α τ₂)
-occurs α (τ₁ | τ₂) = (occurs α τ₁) orelse (occurs α τ₂)
-occurs α (∀ Δ ⟨C⟩ . τ) = 
-  α ∉ Δ andalso
-  (occurs α C) orelse (occurs α τ)
-occurs α (μ β . t) = 
-  α ≠ β andalso 
-  (occurs α τ)
-```
-
-`occurs α C`
-```
-occurs α (τ' ≤ τ) = (occurs α τ') orelse (occurs α τ)
-occurs α (C₁ ∨ C₂) = (occurs α C₁) orelse (occurs α C₂)
-occurs α (C₁ ∧ C₂) = (occurs α C₁) orelse (occurs α C₂)
-```
-
-`subst Δ τ`
-```
-subst Δ α = Δ α 
-subst Δ ? = ? 
-subst Δ [] = [] 
-subst Δ (#l τ) = #l (subst Δ τ) 
-subst Δ (.l τ) = .l (subst Δ τ) 
-subst Δ (τ₁ -> τ₂) = (subst Δ τ₁) -> (subst Δ τ₂)
-subst Δ (τ₁ & τ₂) = (subst Δ τ₁) & (subst Δ τ₂)
-subst Δ (τ₁ | τ₂) = (subst Δ τ₁) | (subst Δ τ₂)
-subst Δ (∀ Δ' ⟨C⟩ . τ) = 
-  let Δ = filter Δ ((α ≤ _)  => α ∉ Δ') in
-  (∀ Δ' ⟨subst Δ C⟩ . (subst Δ τ))
-subst Δ (μ β . τ) = 
-  let Δ = filter Δ ((α ≤ _)  => α ≠ β) in
-  subst Δ (μ β . τ)
-```
-
-`subst Δ C`
-```
-subst Δ (τ' ≤ τ) = (subst Δ τ') ≤ (subst Δ τ)
-subst Δ (C₁ ∨ C₂) = (subst Δ C₁) ∨ (subst Δ C₂)
-subst Δ (C₁ ∧ C₂) = (subst Δ C₁) ∧ (subst Δ C₂)
-```
-
-`unroll μ α . τ = τ`
-```
-unroll μ α . τ = subst {α ≤ μ α . τ} τ
-```
-
-`rename m Δ`
-```
-rename m Δ = 
-  map Δ (α / τ =>
-    let β = m α in
-    {β / subst m τ}
-  )
-```
-
-`guard α τ`
-```
-guard α τ = 
-  μ α . τ
-  if occurs α τ else
-  τ
-```
-
-
-`Δ α = τ` 
-```
-Δ α =  
-  τ
-  if {α → τ} ⊆ Δ else
-  ?
-```
-
-`refresh τ = Δ, C, τ`
-```
-refresh (∀ Δ ⟨C⟩ τ) =
-  let rmap = map Δ (α / _ => {α / fresh}) in
-  let Δ = rename rmap Δ in
-  let C = subst rmap C in
-  let τ = subst rmap τ in
-  Δ, C, τ 
-
-refresh τ = 
-  {}, ., τ
-```
-
-`solve Δ ⊢ C = o[Δ]`
-```
-solve Δ ⊢ C₁ ∧ C₂ =  
-  merge & (solve Δ ⊢ C₁) (solve Δ ⊢ C₂)
-
-solve Δ ⊢ C₁ ∨ C₂ = 
-  merge | (solve Δ ⊢ C₁) (solve Δ ⊢ C₂)
-
-solve Δ ⊢ α ≤ τ =
-  let τ' = Δ α in (
-    let β = fresh in some {α ≤ ((guard α τ) & β), β ≤ ?}
-    if τ' = ? else
-    solve Δ ⊢ τ' ≤ τ
-  )
-
-solve Δ ⊢ τ' ≤ α =
-  let τ = Δ α in (
-    let β = fresh in some {α ≤ ((guard α τ') | β), β ≤ ?}  
-    if τ = ? else
-    (solve Δ ⊢ τ' ≤ τ)
-  )
-
-solve Δ ⊢ (∀ Δ' ⟨C⟩ . τ') ≤ τ =
-  -- quantified Δ' assumed to not be in Δ 
-  map (solve Δ, Δ' ⊢ C ∧ τ' ≤ τ) (Δ'' =>
-    some (map Δ' (α ≤ _ =>
-      {α ≤ Δ''(α)}
-    )) 
-  )
-
-solve Δ ⊢ τ' ≤ (∀ Δ' ⟨C⟩ . τ) =
-  -- quantified Δ' assumed to not be in Δ 
-  map (solve Δ ∪ Δ' ⊢ C ∧ τ' ≤ τ) (Δ'' =>
-    some (map Δ' (α ≤ _ =>
-      {α ≤ Δ''(α)}
-    )) 
-  )
-
-solve Δ ⊢ τ₁ | τ₂ ≤ τ =
-  solve Δ ⊢ τ₁ ≤ τ ∧ τ₂ ≤ τ
-
-solve Δ ⊢ τ ≤ τ₁ | τ₂ =
-  solve Δ ⊢ τ ≤ τ₁ ∨ τ ≤ τ₂
-
-
-solve Δ ⊢ τ ≤ τ₁ & τ₂ =
-  solve Δ ⊢ τ ≤ τ₁ ∧ τ ≤ τ₂
-
-solve Δ ⊢ τ₁ & τ₂ ≤ τ =
-  solve Δ ⊢ τ₁ ≤ τ ∨ τ₂ ≤ τ
-
-solve Δ ⊢ τ₁ -> τ₂' ≤ τ₁' -> τ₂ =
-  solve Δ ⊢ τ₁' ≤ τ₁ ∧ τ₂' ≤ τ₂
-
-
-solve Δ ⊢ #l τ' ≤ μ α . τ =  
-  solve Δ ⊢ #l τ' ≤ unroll (μ α . τ)  
-
-solve Δ ⊢ μ α . τ' ≤ #l τ  =  
-  solve Δ ⊢ unroll (μ α . τ') ≤ #l τ
-
-solve Δ ⊢ .l τ' ≤ μ α . τ =  
-  solve Δ ⊢ .l τ' ≤ unroll (μ α . τ)  
-
-solve Δ ⊢ μ α . τ' ≤ .l τ  =  
-  solve Δ ⊢ unroll (μ α . τ') ≤ .l τ
-
-
-solve Δ ⊢ τ' ≤ μ α . τ =
-  map (linearze_record τ') (τ' =>
-  map (make_field_constraint Δ ⊢ . * τ' ≤ μ α . τ) (C =>
-    solve Δ ⊢ C 
-  ))
-
-solve Δ ⊢ μ α . τ' ≤ τ  =  
-  map (linearze_record τ') (τ' =>
-  map (make_field_constraint Δ ⊢ . * μ α . τ' ≤ τ) (C =>
-    solve Δ ⊢ C 
-  ))
-
-solve Δ ⊢ #l' τ' ≤ #l τ =
-  solve Δ ⊢ τ' ≤ τ
-  if l' = l else
-  none
-
-solve τ ≤ τ = some {} 
-solve _ = none 
-```
-
-`patvars t = o[Γ]`
-```
-patvars x τ = 
-  some {x : τ}
-patvars (.l t₁) τ = 
-  map (project τ l) (τ₁ =>
-    patvars t₁ τ₁
-  )
-patvars (.l t fs) τ =
-  map (patvars (.l t) τ) (Γ₁ =>
-  map (patvars fs τ) (Γ₂ =>
-    some (Γ₁ ∪ Γ₂)
-  ))
-...
-```
-
-`infer Γ Δ ⊢ t : τ = o[Δ;τ]`
-```
-
-infer Γ Δ ⊢ () : τ =
-  map (solve Δ ⊢ C ∧ [] ≤ τ in) (Δ' =>
-    some (Δ' , [])
-  )
-
-infer Γ Δ ⊢ x : τ = 
-  let τ' = Γ x in
-  let Δ', C, τ' = refresh τ' in
-  map (solve Δ, Δ' ⊢ C ∧ τ' ≤ τ) (Δ' =>
-    some (Δ' , τ')
-  )
-
-infer Γ Δ ⊢ (#l t₁) : τ =
-  let α = fresh in
-  map (solve Δ ⊢ (∀ {α} . (#l α)) ≤ τ) (Δ' => 
-  map (infer Γ (Δ ∪ Δ') ⊢ t₁ : α) (Δ₁,τ₁ => 
-    some (Δ' ∪ Δ₁ , #l τ₁)
-  ))
-
-infer Γ Δ ⊢ (for t₁ : τ₁ => t₂) : τ =
-  let Δ₁, τ₁ = τ₁[?/fresh] in
-  let Γ₁ = patvars t₁ τ₁ in
-  let β = fresh in
-  map (solve Δ ⊢ (∀ Δ₁ ∪ {β} . τ₁ -> β) ≤ τ) (Δ' => 
-  map (infer (Γ ∪ Γ₁) (Δ ∪ Δ') ⊢ t₂ : β) (Δ₂', τ₂' =>
-    -- patvars (Γ₁) are NOT generalized in τ₂'
-    some (Δ' ∪ Δ₂' , τ₁ -> τ₂')
-  ))
-
-
-infer Γ Δ ⊢ (for t₁ : τ₁ => t₂) cs : τ =
-  map (infer Γ Δ ⊢ (for t₁ : τ₁ => t₂) : τ) (Δ', τ' =>
-  map (infer Γ Δ ∪ Δ' ⊢ cs : τ₂) (Δ'', τ'' => 
-    some (Δ' ∪ Δ'' , τ' & τ'')
-  ))
-
-infer Γ Δ ⊢ t t₁ : τ₂ =
-  map (infer Γ Δ ⊢ t : ? -> τ₂ in) (Δ',τ' => 
-  map (functify τ') (τ₁,τ₂' => 
-  -- break type (possibly intersection) into premise and conclusion 
-  map (infer Γ (Δ ∪ Δ') ⊢ t₁ : τ₁) (Δ₁',τ₁' =>
-  map (solve Δ ∪ Δ' ∪ Δ₁' ⊢ τ' ≤ (τ₁' -> τ₂)) (Δ' =>
-    some(Δ' , τ₂' & τ₂)
-  ))))
-
-infer Γ Δ ⊢ (.l t₁) : τ =
-  let α = fresh in
-  map (solve Δ ⊢ (∀ {α} . (.l α)) ≤ τ) (Δ' =>
-  map (infer Γ (Δ ∪ Δ') ⊢ t₁ : α) (Δ₁ , τ₁ =>  
-    some(Δ' ∪ Δ₁ , .l τ₁)
-  ))
-
-infer Γ Δ ⊢ (.l t₁) fs : τ =
-  map (infer Γ Δ ⊢ (.l t₁) : τ) (Δ' , τ' =>
-  map (infer Γ (Δ ∪ Δ') ⊢ fs : τ) (Δ'' , τ'' =>
-    some(Δ' ∪ Δ'' , τ' & τ'')
-  ))
-
-infer Γ Δ ⊢ t.l : τ₂ =
-  map (infer Γ Δ ⊢ t : (.l τ₂)) (Δ' , τ' =>
-  map (project τ' l) (τ₂' => 
-    some(Δ' , τ₂')
-  ))
-
-infer Γ Δ ⊢ fix t : τ =
-  map (infer Γ Δ ⊢ t : (τ -> τ)) (Δ',τ' =>
-  map (functify τ') (τ₁', τ₂' =>
-    -- extract premise and conclusion 
-    some(Δ' , τ₂')
-  ))
-
-infer Γ Δ ⊢ (let x : τ₁ = t₁ in t₂) : τ₂ =
-  let Δ₁,τ₁ = τ₁[?/fresh] in
-  map (infer Γ Δ ⊢ t₁ : (∀ Δ₁ . τ₁)) (Δ₁' , τ₁' => 
-  map (infer (Γ ∪ {x : (∀ Δ₁' . τ₁')}) Δ ⊢ t₂ : τ₂) (Δ₂' , τ₂' =>
-    -- τ₁' is generalized in τ₂'
-    some(Δ₂' , τ₂')
-  ))
-```
-
--/
-
--- static implementation/semantics theorems
-/-
-soundness: ...
-completeness: ...
--/
-
-
--- static/dynamic semantics theorems
-/-
-soundness: N/A
-completeness: N/A
--/
-
-
